many changes

src/sable_verified.cpp
@@ -7,9 +7,18 @@
 # 1 "/Users/scottconstable/Documents/SU_Graduate/SABLE/sable/src/sable_verified.c" 2
 # 1 "/Users/scottconstable/Documents/SU_Graduate/SABLE/sable/build/include/sable_verified.h" 1
 
-void trusted_boot(void);
+void reboot(void)__attribute__((noreturn));
 typedef unsigned long UINT32;
+UINT32 memcmp(const void *buf1,const void *buf2,UINT32 size);
+void trusted_boot(void);
+typedef struct TPM_Unseal_ret TPM_Unseal_ret;
 typedef UINT32 TPM_RESULT;
+typedef unsigned char BYTE;
+struct TPM_Unseal_ret {
+  TPM_RESULT returnCode;
+  UINT32 dataSize;
+  BYTE *data;
+};
 typedef struct tdTPM_STORED_DATA12 tdTPM_STORED_DATA12;
 typedef unsigned short UINT16;
 typedef UINT16 TPM_STRUCTURE_TAG;
@@ -20,7 +29,6 @@ typedef UINT16 TPM_ENTITY_TYPE;
 
 
 
-typedef unsigned char BYTE;
 struct tdTPM_STORED_DATA12 {
   TPM_STRUCTURE_TAG tag;
   TPM_ENTITY_TYPE et;
@@ -48,18 +56,30 @@ struct tdTPM_NONCE {
 };
 typedef struct tdTPM_NONCE TPM_NONCE;
 typedef BYTE TPM_BOOL;
+typedef struct tdTPM_OSAP_EXTENSION tdTPM_OSAP_EXTENSION;
+struct tdTPM_OSAP_EXTENSION {
+  TPM_NONCE nonceEvenOSAP;
+  TPM_NONCE nonceOddOSAP;
+};
+typedef struct tdTPM_OSAP_EXTENSION TPM_OSAP_EXTENSION;
 struct tdTPM_SESSION {
   TPM_AUTHHANDLE authHandle;
   TPM_NONCE nonceEven;
   TPM_NONCE nonceOdd;
   TPM_BOOL continueAuthSession;
+  TPM_OSAP_EXTENSION *osap;
 };
 typedef struct tdTPM_SESSION TPM_SESSION;
-TPM_RESULT TPM_Unseal(TPM_STORED_DATA12 inData_in,BYTE *secret_out,UINT32 secretSizeMax,TPM_KEY_HANDLE parentHandle_in,TPM_AUTHDATA parentAuth,TPM_SESSION *parentSession,TPM_AUTHDATA dataAuth,TPM_SESSION *dataSession);
-void unseal_passphrase(TPM_AUTHDATA srk_auth,TPM_AUTHDATA pp_auth,TPM_STORED_DATA12 sealed_pp);
+struct TPM_Unseal_ret TPM_Unseal(TPM_STORED_DATA12 inData_in,TPM_KEY_HANDLE parentHandle_in,TPM_AUTHDATA parentAuth,TPM_SESSION **parentSession,TPM_AUTHDATA dataAuth,TPM_SESSION **dataSession);
+const char *unseal_passphrase(TPM_AUTHDATA srk_auth,TPM_AUTHDATA pp_auth,TPM_STORED_DATA12 sealed_pp);
 TPM_STORED_DATA12 unpack_TPM_STORED_DATA12(const BYTE *data,UINT32 dataSize);
 
-
+typedef struct TPM_NV_ReadValue_ret TPM_NV_ReadValue_ret;
+struct TPM_NV_ReadValue_ret {
+  TPM_RESULT returnCode;
+  UINT32 dataSize;
+  BYTE *data;
+};
 typedef UINT32 TPM_NV_INDEX;
 
 
@@ -73,7 +93,7 @@ struct TPM_AUTHDATA_option { TPM_AUTHDATA value; char hasValue; };
 
 
 
-TPM_RESULT TPM_NV_ReadValue(BYTE *data_out,TPM_NV_INDEX nvIndex_in,UINT32 offset_in,UINT32 dataSize_in,struct TPM_AUTHDATA_option ownerAuth_in,TPM_SESSION *session);
+struct TPM_NV_ReadValue_ret TPM_NV_ReadValue(TPM_NV_INDEX nvIndex_in,UINT32 offset_in,UINT32 dataSize_in,struct TPM_AUTHDATA_option ownerAuth_in,TPM_SESSION **session);
 TPM_STORED_DATA12 read_passphrase(void);
 
 
@@ -88,9 +108,15 @@ void out_string(const char *value);
 
 
 void configure(void);
-TPM_RESULT TPM_NV_WriteValueAuth(const BYTE *data_in,UINT32 dataSize_in,TPM_NV_INDEX nvIndex_in,UINT32 offset_in,TPM_AUTHDATA nv_auth,TPM_SESSION *session);
-TPM_RESULT TPM_OIAP(TPM_SESSION *session);
-void write_passphrase(TPM_AUTHDATA nv_auth);
+TPM_RESULT TPM_NV_WriteValueAuth(const BYTE *data_in,UINT32 dataSize_in,TPM_NV_INDEX nvIndex_in,UINT32 offset_in,TPM_AUTHDATA nv_auth,TPM_SESSION **session);
+typedef struct extracted_TPM_STORED_DATA12 extracted_TPM_STORED_DATA12;
+struct extracted_TPM_STORED_DATA12 {
+  UINT32 dataSize;
+  BYTE *data;
+};
+struct extracted_TPM_STORED_DATA12 extract_TPM_STORED_DATA12(TPM_STORED_DATA12 storedData);
+TPM_RESULT TPM_OIAP(TPM_SESSION **session);
+void write_passphrase(TPM_AUTHDATA nv_auth,TPM_STORED_DATA12 sealedData);
 typedef struct TPM_Seal_ret TPM_Seal_ret;
 struct TPM_Seal_ret {
   TPM_RESULT returnCode;
@@ -121,7 +147,7 @@ struct tdTPM_PCR_INFO_LONG {
 };
 typedef struct tdTPM_PCR_INFO_LONG TPM_PCR_INFO_LONG;
 typedef TPM_AUTHDATA TPM_SECRET;
-struct TPM_Seal_ret TPM_Seal(BYTE *rawData,UINT32 rawDataSize,TPM_KEY_HANDLE keyHandle_in,TPM_ENCAUTH encAuth_in,TPM_PCR_INFO_LONG pcrInfo_in,const BYTE *inData_in,UINT32 inDataSize_in,TPM_SESSION *session,TPM_SECRET sharedSecret);
+struct TPM_Seal_ret TPM_Seal(TPM_KEY_HANDLE keyHandle_in,TPM_ENCAUTH encAuth_in,TPM_PCR_INFO_LONG pcrInfo_in,const BYTE *inData_in,UINT32 inDataSize_in,TPM_SESSION **session,TPM_SECRET sharedSecret);
 TPM_ENCAUTH encAuth_gen(TPM_AUTHDATA entityAuthData,TPM_SECRET sharedSecret,TPM_NONCE authLastNonceEven);
 TPM_SECRET sharedSecret_gen(TPM_AUTHDATA auth,TPM_NONCE nonceEvenOSAP,TPM_NONCE nonceOddOSAP);
 
@@ -129,15 +155,8 @@ TPM_SECRET sharedSecret_gen(TPM_AUTHDATA auth,TPM_NONCE nonceEvenOSAP,TPM_NONCE 
 
 
 
-typedef struct tdTPM_OSAP_SESSION tdTPM_OSAP_SESSION;
-struct tdTPM_OSAP_SESSION {
-  TPM_SESSION session;
-  TPM_NONCE nonceEvenOSAP;
-  TPM_NONCE nonceOddOSAP;
-};
-typedef struct tdTPM_OSAP_SESSION TPM_OSAP_SESSION;
-TPM_RESULT TPM_OSAP(TPM_ENTITY_TYPE entityType_in,UINT32 entityValue_in,TPM_OSAP_SESSION *osap_session);
-void seal_passphrase(TPM_AUTHDATA srk_auth,TPM_AUTHDATA pp_auth,UINT32 lenPassphrase);
+TPM_RESULT TPM_OSAP(TPM_ENTITY_TYPE entityType_in,UINT32 entityValue_in,TPM_NONCE nonceOddOSAP,TPM_SESSION **session);
+TPM_STORED_DATA12 seal_passphrase(TPM_AUTHDATA srk_auth,TPM_AUTHDATA pp_auth,const char *passphrase,UINT32 lenPassphrase);
 
 
 typedef struct tdTPM_PCR_COMPOSITE tdTPM_PCR_COMPOSITE;
@@ -150,11 +169,11 @@ struct tdTPM_PCR_COMPOSITE {
 };
 typedef struct tdTPM_PCR_COMPOSITE TPM_PCR_COMPOSITE;
 TPM_COMPOSITE_HASH get_TPM_COMPOSITE_HASH(TPM_PCR_COMPOSITE comp);
-# 153 "/Users/scottconstable/Documents/SU_Graduate/SABLE/sable/build/include/sable_verified.h"
+# 172 "/Users/scottconstable/Documents/SU_Graduate/SABLE/sable/build/include/sable_verified.h"
 const char *tpm_error_to_string(TPM_RESULT res);
 void wait(int ms);
 void exit(unsigned status)__attribute__((noreturn));
-# 164 "/Users/scottconstable/Documents/SU_Graduate/SABLE/sable/build/include/sable_verified.h"
+# 183 "/Users/scottconstable/Documents/SU_Graduate/SABLE/sable/build/include/sable_verified.h"
 typedef struct TPM_PCRRead_ret TPM_PCRRead_ret;
 struct TPM_PCRRead_ret {
   TPM_RESULT returnCode;
@@ -162,41 +181,46 @@ struct TPM_PCRRead_ret {
 };
 typedef UINT32 TPM_PCRINDEX;
 struct TPM_PCRRead_ret TPM_PCRRead(TPM_PCRINDEX pcrIndex_in);
+void *alloc(UINT32 size);
 TPM_PCR_INFO_LONG get_pcr_info(void);
+
 TPM_NONCE get_nonce(void);
 TPM_AUTHDATA get_authdata(void);
+typedef struct tdTPM_SEALED_DATA tdTPM_SEALED_DATA;
+typedef BYTE TPM_PAYLOAD_TYPE;
+struct tdTPM_SEALED_DATA {
+  TPM_PAYLOAD_TYPE payload;
+  TPM_SECRET authData;
+  TPM_SECRET tpmProof;
+  TPM_DIGEST storedDigest;
+  UINT32 dataSize;
+
+  BYTE *data;
+};
+typedef struct tdTPM_SEALED_DATA TPM_SEALED_DATA;
 # 2 "/Users/scottconstable/Documents/SU_Graduate/SABLE/sable/src/sable_verified.c" 2
 
 
 
 
+typedef TPM_SEALED_DATA
+    BOGUS1;
+
 extern TPM_AUTHDATA get_authdata(void);
 extern TPM_NONCE get_nonce(void);
 
-
-
-
-
-static char passphrase[128];
-static BYTE pp_blob[400];
-static BYTE pcr_select_bytes[3] = {0x0, 0x0, 0xa};
-static const TPM_PCR_SELECTION pcr_select = {
-    .sizeOfSelect = sizeof(pcr_select_bytes),
-    .pcrSelect = (BYTE *)pcr_select_bytes};
-static TPM_PCRVALUE pcr_values[2];
-
-
-static TPM_OSAP_SESSION srk_osap_session;
-static TPM_SESSION nv_session;
-static TPM_SESSION srk_session;
-static TPM_SESSION pp_session;
-
-
-
+static TPM_SESSION *sessions[2] = {0, 0};
 
 
 
 TPM_PCR_INFO_LONG get_pcr_info(void) {
+  TPM_PCRVALUE *pcr_values = alloc(2 * sizeof(TPM_PCRVALUE));
+  BYTE *pcr_select_bytes = alloc(3);
+  pcr_select_bytes[0] = 0x00;
+  pcr_select_bytes[1] = 0x00;
+  pcr_select_bytes[2] = 0x0a;
+  TPM_PCR_SELECTION pcr_select = {.sizeOfSelect = 3,
+                                  .pcrSelect = (BYTE *)pcr_select_bytes};
   struct TPM_PCRRead_ret pcr17 = TPM_PCRRead(17);
   { if (pcr17.returnCode) { ; exit(pcr17.returnCode); } };
   pcr_values[0] = pcr17.outDigest;
@@ -204,7 +228,7 @@ TPM_PCR_INFO_LONG get_pcr_info(void) {
   { if (pcr19.returnCode) { ; exit(pcr19.returnCode); } };
   pcr_values[1] = pcr19.outDigest;
   TPM_PCR_COMPOSITE composite = {.select = pcr_select,
-                                 .valueSize = sizeof(pcr_values),
+                                 .valueSize = 2 * sizeof(TPM_PCRVALUE),
                                  .pcrValue = (TPM_PCRVALUE *)pcr_values};
   TPM_COMPOSITE_HASH composite_hash = get_TPM_COMPOSITE_HASH(composite);
   TPM_PCR_INFO_LONG pcr_info = {.tag = ((UINT16)0x0006),
@@ -217,54 +241,60 @@ TPM_PCR_INFO_LONG get_pcr_info(void) {
   return pcr_info;
 }
 
-void seal_passphrase(TPM_AUTHDATA srk_auth, TPM_AUTHDATA pp_auth,
-                     UINT32 lenPassphrase) {
+TPM_STORED_DATA12 seal_passphrase(TPM_AUTHDATA srk_auth, TPM_AUTHDATA pp_auth,
+                                  const char *passphrase,
+                                  UINT32 lenPassphrase) {
   TPM_RESULT res;
 
 
-  srk_osap_session.nonceOddOSAP = get_nonce();
-  res = TPM_OSAP(((UINT16)0x0001), ((UINT32)0x40000000), &srk_osap_session);
+  TPM_NONCE nonceOddOSAP = get_nonce();
+  res = TPM_OSAP(((UINT16)0x0001), ((UINT32)0x40000000), nonceOddOSAP, &sessions[0]);
   { if (res) { ; exit(res); } };
-  srk_osap_session.session.continueAuthSession = 0x00;
+  sessions[0]->nonceOdd = get_nonce();
+  sessions[0]->continueAuthSession = 0x00;
 
 
-  TPM_SECRET sharedSecret = sharedSecret_gen(
-      srk_auth, srk_osap_session.nonceEvenOSAP, srk_osap_session.nonceOddOSAP);
-
-
-  srk_osap_session.session.nonceOdd = get_nonce();
+  TPM_SECRET sharedSecret =
+      sharedSecret_gen(srk_auth, sessions[0]->osap->nonceEvenOSAP,
+                       sessions[0]->osap->nonceOddOSAP);
 
 
   TPM_ENCAUTH encAuth =
-      encAuth_gen(pp_auth, sharedSecret, srk_osap_session.session.nonceEven);
+      encAuth_gen(pp_auth, sharedSecret, sessions[0]->nonceEven);
 
   TPM_PCR_INFO_LONG pcr_info = get_pcr_info();
 
 
   struct TPM_Seal_ret seal_ret =
-      TPM_Seal(pp_blob, sizeof(pp_blob), ((UINT32)0x40000000), encAuth, pcr_info,
-               (const BYTE *)passphrase, lenPassphrase,
-               &srk_osap_session.session, sharedSecret);
+      TPM_Seal(((UINT32)0x40000000), encAuth, pcr_info, (const BYTE *)passphrase,
+               lenPassphrase, &sessions[0], sharedSecret);
   { if (seal_ret.returnCode) { ; exit(seal_ret.returnCode); } };
+
+  return seal_ret.sealedData;
 }
 
-void write_passphrase(TPM_AUTHDATA nv_auth) {
+void write_passphrase(TPM_AUTHDATA nv_auth, TPM_STORED_DATA12 sealedData) {
   TPM_RESULT res;
 
-  res = TPM_OIAP(&nv_session);
+  res = TPM_OIAP(&sessions[0]);
   { if (res) { ; exit(res); } };
+  sessions[0]->nonceOdd = get_nonce();
+  sessions[0]->continueAuthSession = 0x00;
 
-  res = TPM_NV_WriteValueAuth(pp_blob, sizeof(pp_blob), 0x04, 0, nv_auth,
-                              &nv_session);
+  struct extracted_TPM_STORED_DATA12 x = extract_TPM_STORED_DATA12(sealedData);
+  res =
+      TPM_NV_WriteValueAuth(x.data, x.dataSize, 0x04, 0, nv_auth, &sessions[0]);
   { if (res) { ; exit(res); } };
 }
 
 void configure(void) {
+  char *passphrase = alloc(128);
+
 
 
 
   UINT32 lenPassphrase =
-      get_string(passphrase, sizeof(passphrase) - 1, 1) + 1;
+      get_string(passphrase, 128 - 1, 1) + 1;
 
 
   TPM_AUTHDATA pp_auth = get_authdata();
@@ -273,41 +303,48 @@ void configure(void) {
   TPM_AUTHDATA srk_auth = get_authdata();
 
 
-  seal_passphrase(srk_auth, pp_auth, lenPassphrase);
+  TPM_STORED_DATA12 sealedData =
+      seal_passphrase(srk_auth, pp_auth, passphrase, lenPassphrase);
 
 
 
   TPM_AUTHDATA nv_auth = get_authdata();
 
 
-  write_passphrase(nv_auth);
+  write_passphrase(nv_auth, sealedData);
 }
 
 TPM_STORED_DATA12 read_passphrase(void) {
-  TPM_RESULT res;
+  struct TPM_NV_ReadValue_ret val;
   struct TPM_AUTHDATA_option nv_auth;
 # 136 "/Users/scottconstable/Documents/SU_Graduate/SABLE/sable/src/sable_verified.c"
   nv_auth.hasValue = 0;
-  res = TPM_NV_ReadValue(pp_blob, 4, 0, sizeof(pp_blob), nv_auth, 0);
-  { if (res) { ; exit(res); } };
+  val = TPM_NV_ReadValue(4, 0, 400, nv_auth, 0);
+  { if (val.returnCode) { ; exit(val.returnCode); } };
 
 
-  return unpack_TPM_STORED_DATA12(pp_blob, sizeof(pp_blob));
+  return unpack_TPM_STORED_DATA12(val.data, val.dataSize);
 }
 
-void unseal_passphrase(TPM_AUTHDATA srk_auth, TPM_AUTHDATA pp_auth,
-                       TPM_STORED_DATA12 sealed_pp) {
+const char *unseal_passphrase(TPM_AUTHDATA srk_auth, TPM_AUTHDATA pp_auth,
+                              TPM_STORED_DATA12 sealed_pp) {
   TPM_RESULT res;
 
-  res = TPM_OIAP(&srk_session);
+  res = TPM_OIAP(&sessions[0]);
   { if (res) { ; exit(res); } };
+  sessions[0]->nonceOdd = get_nonce();
+  sessions[0]->continueAuthSession = 0x00;
 
-  res = TPM_OIAP(&pp_session);
+  res = TPM_OIAP(&sessions[1]);
   { if (res) { ; exit(res); } };
+  sessions[1]->nonceOdd = get_nonce();
+  sessions[1]->continueAuthSession = 0x00;
 
-  res = TPM_Unseal(sealed_pp, (BYTE *)passphrase, sizeof(passphrase), ((UINT32)0x40000000),
-                   srk_auth, &srk_session, pp_auth, &pp_session);
-  { if (res) { ; exit(res); } };
+  TPM_Unseal_ret unseal_ret = TPM_Unseal(sealed_pp, ((UINT32)0x40000000), srk_auth,
+                                         &sessions[0], pp_auth, &sessions[1]);
+  { if (unseal_ret.returnCode) { ; exit(unseal_ret.returnCode); } };
+
+  return (const char *)unseal_ret.data;
 }
 
 void trusted_boot(void) {
@@ -320,6 +357,6 @@ void trusted_boot(void) {
 
   TPM_AUTHDATA srk_auth = get_authdata();
 
-  unseal_passphrase(srk_auth, pp_auth, sealed_pp);
-# 211 "/Users/scottconstable/Documents/SU_Graduate/SABLE/sable/src/sable_verified.c"
+  const char *passphrase = unseal_passphrase(srk_auth, pp_auth, sealed_pp);
+# 185 "/Users/scottconstable/Documents/SU_Graduate/SABLE/sable/src/sable_verified.c"
 }
