Abstract/AMonad.thy
@@ -1,7 +1,7 @@
 theory AMonad
 imports
   "../lib/NondetExtensions"
-  TPM
+  "../Machine/Machine"
 begin
 
 record Session =
@@ -10,9 +10,9 @@ record Session =
   continue :: bool
 
 definition
-  Session_empty :: "(TPM.AUTHHANDLE, Session) lookup"
+  empty_Session :: "(TPM.AUTHHANDLE, Session) lookup"
 where
-  "Session_empty \<equiv> \<lambda>_. None"
+  "empty_Session \<equiv> \<lambda>_. None"
 
 definition
   update_Session :: "(TPM.AUTHHANDLE, Session) lookup \<Rightarrow> TPM.AUTHHANDLE \<Rightarrow> Session
@@ -21,26 +21,36 @@ where
   "update_Session m h s \<equiv> \<lambda>h'. if h' = h then Some s else m h'"
 
 record astate =
-  powerOn :: bool
+  machine :: machine_state
   sessions :: "(TPM.AUTHHANDLE, Session) lookup"
-  tpm :: tpm_state
 
 type_synonym 'a s_monad = "(astate, 'a) nondet_monad"
 
 definition
-  tpm_lift :: "'a tpm_monad \<Rightarrow> 'a s_monad"
+  machine_op_lift :: "'a machine_monad \<Rightarrow> 'a s_monad"
 where
-  "tpm_lift m \<equiv>
+  "machine_op_lift m \<equiv>
    do
-    tpm_state \<leftarrow> gets tpm;
-    (r, tpm_state') \<leftarrow> select_f (m tpm_state);
-    modify (\<lambda>s. s \<lparr> tpm := tpm_state' \<rparr>);
+    mstate \<leftarrow> gets machine;
+    (r, tpm_state') \<leftarrow> select_f (m mstate);
+    modify (\<lambda>s. s \<lparr> machine := mstate \<rparr>);
     return r
    od"
 
+definition "m_tpm_lift \<equiv> machine_op_lift \<circ> tpm_lift"
+
 definition
-  reboot :: "unit s_monad"
+  exit :: "unit s_monad"
 where
-  "reboot \<equiv> modify (\<lambda>s. s\<lparr> powerOn := False \<rparr>)"
+  "exit \<equiv> machine_op_lift $ modify (\<lambda>s. s\<lparr> powerOn := False \<rparr>)"
+
+definition
+  exit_r :: "'a s_monad"
+where
+  "exit_r \<equiv>
+   do
+    exit;
+    unknown
+   od"
 
 end
