Abstract/Abstract.thy
@@ -4,35 +4,20 @@ imports
   TPM_Driver
 begin
 
-(*definition
-  exit :: "unit s_monad"
+definition
+  get_authdata :: "TPM.AUTHDATA s_monad"
 where
-  "exit \<equiv> \<lambda>s. ({}, False)"
+  "get_authdata \<equiv> unknown"
 
 definition
-  getAuthData :: "auth_data s_monad"
+  get_nonce :: "TPM.NONCE s_monad"
 where
-  "getAuthData \<equiv>
-   do
-    auth \<leftarrow> select UNIV;
-    return auth
-   od"
+  "get_nonce \<equiv> unknown"
 
 definition
-  authorize :: "auth_data \<Rightarrow> (device_error + unit) s_monad"
+  read_passphrase :: "(string TPM.STORED_DATA) s_monad"
 where
-  "authorize auth \<equiv> select UNIV"
-
-definition
-  main :: "int s_monad"
-where
-  "main \<equiv>
-   do
-    auth \<leftarrow> getAuthData;
-    authorize auth
-    <catch> (\<lambda>_. exit);
-    return 0
-   od"
+  "read_passphrase \<equiv> TPM_NV_ReadValue 4 0 None <catch> (\<lambda>e. exit_r)"
 
 definition
   A_proc :: "(astate, astate) data_type"
@@ -40,7 +25,7 @@ where
   "A_proc \<equiv> \<lparr>
     Init = \<lambda>s. {s},
     Fin = id,
-    Run = lift_nd main
-  \<rparr>"*)
+    Run = lift_nd read_passphrase
+  \<rparr>"
 
 end
