Machine/Machine.thy
@@ -1,0 +1,23 @@
+theory Machine
+imports
+  TPM
+begin
+
+record machine_state =
+  powerOn :: bool
+  tpm :: tpm_state
+
+type_synonym 'a machine_monad = "(machine_state, 'a) nondet_monad"
+
+definition
+  tpm_lift :: "'a tpm_monad \<Rightarrow> 'a machine_monad"
+where
+  "tpm_lift m \<equiv>
+   do
+    tpm_state \<leftarrow> gets tpm;
+    (r, tpm_state') \<leftarrow> select_f (m tpm_state);
+    modify (\<lambda>s. s \<lparr> tpm := tpm_state' \<rparr>);
+    return r
+   od"
+
+end
