Machine/TPM.thy
@@ -1,0 +1,276 @@
+theory TPM
+imports
+  "../lib/NondetExtensions"
+begin
+
+datatype 'a Enc = encrypt 'a
+
+(* External Structures, from TPM Main Part 2 *)
+
+datatype PCRINDEX = PCR0 | PCR1 | PCR2 | PCR3 | PCR4 | PCR5 | PCR6 | PCR7 | PCR8 | PCR9 | PCR10
+| PCR11 | PCR12 | PCR13 | PCR14 | PCR15 | PCR16 | PCR17 | PCR18 | PCR19 | PCR20 | PCR21 | PCR22
+| PCR23
+type_synonym PCR_SELECTION = "PCRINDEX set"
+
+datatype LOCALITY = LOC_ZERO | LOC_ONE | LOC_TWO | LOC_THREE | LOC_FOUR
+type_synonym LOCALITY_SELECTION = "LOCALITY set"
+
+type_synonym NV_INDEX = nat
+
+datatype ERROR = AUTHFAIL | OTHER_ERROR
+
+type_synonym RESULT = "ERROR + unit"
+type_synonym AUTHHANDLE = nat
+
+datatype NONCE = nonce nat
+
+(* FIXME: fill this in? *)
+typedecl ENTITY_TYPE
+
+(* FIXME: fill this in? *)
+datatype PAYLOAD_TYPE = PT_SEAL
+
+(* helper type *)
+datatype dig =
+  PCRINDEX_dig PCRINDEX
+| PCR_SELECTION_dig PCR_SELECTION
+| NV_INDEX_dig NV_INDEX
+| RESULT_dig RESULT
+| AUTHHANDLE_dig AUTHHANDLE
+| AUTHDATA_dig AUTHDATA
+| NONCE_dig NONCE
+| ENTITY_TYPE_dig ENTITY_TYPE
+| PAYLOAD_TYPE_dig PAYLOAD_TYPE
+| LOCALITY_SELECTION_dig LOCALITY_SELECTION
+| char_dig char
+| nat_dig nat
+| bool_dig bool
+| DIGEST_dig "dig list"
+| Enc_dig (* hash of encrypted data *)
+and AUTHDATA = auth nat | hmac AUTHDATA "dig list"
+
+type_synonym DIGEST = "dig list"
+
+(* Hashable instances for atomic types *)
+
+class Hashable =
+  fixes hash :: "'a \<Rightarrow> DIGEST"
+  assumes injective: "hash x = hash y \<Longrightarrow> x = y"
+
+instantiation unit :: Hashable
+begin
+definition "hash_unit \<equiv> \<lambda>_ :: unit. Nil :: DIGEST"
+instance proof
+  fix x y :: unit
+  assume "hash x = hash y"
+  thus "x = y" by auto
+qed
+end
+
+instantiation char :: Hashable
+begin
+definition "hash_char c \<equiv> [char_dig c]"
+instance proof
+  fix x y :: char
+  assume "hash x = hash y"
+  thus "x = y" unfolding hash_char_def by simp
+qed
+end
+
+instantiation list :: (Hashable) Hashable
+begin
+definition "hash_list = map (DIGEST_dig \<circ> hash)"
+instance proof
+  fix xs ys :: "'a list"
+  assume "hash xs = hash ys"
+  thus "xs = ys" unfolding hash_list_def
+  proof (induction ys arbitrary: xs)
+    case Nil thus "xs = []" by simp
+  next
+    fix y :: 'a and xs'' ys' :: "'a list"
+    assume IH: "\<And>xs. map (DIGEST_dig \<circ> hash) xs = map (DIGEST_dig \<circ> hash) ys' \<Longrightarrow> xs = ys'"
+       and xs'': "map (DIGEST_dig \<circ> hash) xs'' = map (DIGEST_dig \<circ> hash) (y # ys')"
+    { assume "xs'' = Nil"
+      with xs'' have False by auto
+      hence "xs'' = y # ys'" .. }
+    moreover
+    { fix x xs'
+      assume a: "xs'' = x # xs'"
+      with xs'' have "map (DIGEST_dig \<circ> hash) xs' = map (DIGEST_dig \<circ> hash) ys'" by simp
+      hence "xs' = ys'" using IH by auto
+      hence "x # xs' = y # ys'" using xs'' a and injective by auto
+      with a have "xs'' = y # ys'" by simp }
+    ultimately show "xs'' = y # ys'" using xs'' by auto
+  qed
+qed
+end
+
+instantiation Enc :: (Hashable) Hashable
+begin
+definition "hash_Enc e \<equiv> case e of encrypt d \<Rightarrow> [Enc_dig, DIGEST_dig (hash d)]"
+instance proof
+  fix x y :: "('a :: Hashable) Enc"
+  assume "hash x = hash y"
+  thus "x = y" unfolding hash_Enc_def
+    apply (case_tac x)
+    apply (case_tac y)
+    apply (simp add: injective)
+    done
+qed
+end
+
+(* derived TPM types *)
+
+record PCR_INFO_LONG =
+  localityAtCreation :: LOCALITY_SELECTION
+  localityAtRelease :: LOCALITY_SELECTION
+  creationPCRSelection :: PCR_SELECTION
+  releasePCRSelection :: PCR_SELECTION
+  digestAtCreation :: DIGEST
+  digestAtRelease :: DIGEST
+
+instantiation PCR_INFO_LONG_ext :: (Hashable) Hashable
+begin
+
+definition "hash_PCR_INFO_LONG_ext i \<equiv>
+  [LOCALITY_SELECTION_dig (localityAtCreation i),
+   LOCALITY_SELECTION_dig (localityAtRelease i),
+   PCR_SELECTION_dig (creationPCRSelection i),
+   PCR_SELECTION_dig (releasePCRSelection i),
+   DIGEST_dig (digestAtCreation i),
+   DIGEST_dig (digestAtRelease i),
+   DIGEST_dig (hash (more i))]"
+
+instance proof
+  fix x y :: "('a :: Hashable) PCR_INFO_LONG_scheme"
+  assume "hash x = hash y"
+  thus "x = y" unfolding hash_PCR_INFO_LONG_ext_def by (simp add: injective)
+qed
+
+end
+
+record ('a :: Hashable) SEALED_DATA =
+  payload :: PAYLOAD_TYPE
+  authData :: AUTHDATA
+  tpmProof :: AUTHDATA
+  storedDigest :: DIGEST
+  data :: 'a
+
+instantiation SEALED_DATA_ext :: (Hashable, Hashable) Hashable
+begin
+
+definition "hash_SEALED_DATA_ext d \<equiv>
+  [PAYLOAD_TYPE_dig (payload d),
+   AUTHDATA_dig (authData d),
+   AUTHDATA_dig (tpmProof d),
+   DIGEST_dig (storedDigest d),
+   DIGEST_dig (hash (data d)),
+   DIGEST_dig (hash (more d))]"
+
+instance proof
+  fix x y :: "('a :: Hashable, 'z :: Hashable) SEALED_DATA_scheme"
+  assume "hash x = hash y"
+  thus "x = y" unfolding hash_SEALED_DATA_ext_def by (simp add: injective)
+qed
+
+end
+
+record ('a :: Hashable) STORED_DATA =
+  et :: ENTITY_TYPE
+  pcrInfo :: PCR_INFO_LONG
+  encData :: "('a SEALED_DATA) Enc"
+
+instantiation STORED_DATA_ext :: (Hashable, Hashable) Hashable
+begin
+
+definition "hash_STORED_DATA_ext d \<equiv>
+  [ENTITY_TYPE_dig (et d),
+   DIGEST_dig (hash (pcrInfo d)),
+   DIGEST_dig (hash (encData d)),
+   DIGEST_dig (hash (more d))]"
+
+instance proof
+  fix x y :: "('a :: Hashable, 'z :: Hashable) STORED_DATA_scheme"
+  assume "hash x = hash y"
+  thus "x = y" unfolding hash_STORED_DATA_ext_def by (simp add: injective)
+qed
+
+end
+
+(* auxiliary TPM Structures *)
+
+record Auth_in =
+  authHandle :: AUTHHANDLE
+  nonceOdd :: NONCE
+  continueAuthSession :: bool
+  auth :: AUTHDATA
+
+record Auth_out =
+  nonceEven :: NONCE
+  continueAuthSession :: bool
+  auth :: AUTHDATA
+
+(* TPM State representation *)
+
+(*record Session =
+  nonceEven :: NONCE
+  nonceOdd :: "NONCE option"
+
+type_synonym Session_map = "AUTHHANDLE \<Rightarrow> Session option"
+
+definition
+  Session_empty :: Session_map
+where
+  "Session_empty \<equiv> \<lambda>_. None"
+
+definition
+  update_Session :: "Session_map \<Rightarrow> AUTHHANDLE \<Rightarrow> Session \<Rightarrow> Session_map"
+where
+  "update_Session m h s \<equiv> \<lambda>h'. if h' = h then Some s else m h'"
+
+record tpm_state =
+  sessions :: Session_map*)
+
+type_synonym tpm_state = unit
+type_synonym 'a tpm_monad = "(tpm_state, 'a) nondet_monad"
+
+(* TPM Commands, from TPM Main Part 3 *)
+
+record PCRRead_in =
+  pcrIndex :: PCRINDEX
+
+record PCRRead_out =
+  returnCode :: RESULT
+  outDigest :: DIGEST
+
+definition
+  PCRRead :: "PCRRead_in \<Rightarrow> PCRRead_out tpm_monad"
+where
+  "PCRRead com \<equiv> select (UNIV :: PCRRead_out set)"
+
+record OIAP_out =
+  returnCode :: RESULT
+  authHandle :: AUTHHANDLE
+  nonceEven :: NONCE
+
+definition
+  OIAP :: "OIAP_out tpm_monad"
+where
+  "OIAP \<equiv> unknown"
+
+record NV_ReadValue_in =
+  nvIndex :: NV_INDEX
+  offset :: nat
+  ownerAuth :: "Auth_in option"
+
+record 'a NV_ReadValue_out =
+  returnCode :: RESULT
+  data :: 'a
+  ownerAuth :: Auth_out
+
+definition
+  NV_ReadValue :: "NV_ReadValue_in \<Rightarrow> ('a NV_ReadValue_out) tpm_monad"
+where
+  "NV_ReadValue com \<equiv> unknown"
+
+end
