Proofs/RRelation.thy
@@ -9,6 +9,20 @@ where
   "TPM_PCRRead_rel r r' \<equiv>
     case r of
       Inl error \<Rightarrow> ERROR_rel error (TPM_PCRRead_ret_C.returnCode_C r')
-    | Inr digest \<Rightarrow> DIGEST_rel digest (TPM_PCRRead_ret_C.outDigest_C r')"
+    | Inr digest \<Rightarrow> TPM_PCRRead_ret_C.returnCode_C r' = 0 \<and>
+        DIGEST_rel digest (TPM_PCRRead_ret_C.outDigest_C r')"
+
+definition
+  TPM_NV_ReadValue_rel :: "(('a :: Hashable) \<Rightarrow> (8 word ptr \<times> 32 word) \<times> lifted_globals \<Rightarrow> bool)
+                          \<Rightarrow> TPM.ERROR + 'a
+                          \<Rightarrow> TPM_NV_ReadValue_ret_C \<times> lifted_globals
+                          \<Rightarrow> bool"
+where
+  "TPM_NV_ReadValue_rel vrel r r' \<equiv>
+    case r of
+      Inl e \<Rightarrow> ERROR_rel e (TPM_NV_ReadValue_ret_C.returnCode_C (fst r'))
+    | Inr v \<Rightarrow> TPM_NV_ReadValue_ret_C.returnCode_C (fst r') = TPM_SUCCESS \<and>
+        vrel v ((TPM_NV_ReadValue_ret_C.data_C (fst r'),
+        TPM_NV_ReadValue_ret_C.dataSize_C (fst r')), snd r')"
 
 end
