Proofs/Refine_AC_A.thy
@@ -1,23 +1,97 @@
 theory Refine_AC_A
 imports
-  "../AutoCorres/Impl"
-  "../Abstract/Abstract"
-  "../lib/NondetCorres"
+  TPM_Corres
 begin
 
-definition "R \<equiv> UNIV :: (astate \<times> lifted_globals) set"
-definition "I\<^sub>C \<equiv> UNIV :: lifted_globals set"
-definition "I\<^sub>A \<equiv> UNIV :: astate set"
+context sable_m
+begin
 
-(*lemma corres: "corres_underlying R False True \<top>\<top>
-  (\<lambda>s\<^sub>A. s\<^sub>A \<in> I\<^sub>A) (\<lambda>s\<^sub>C. s\<^sub>C \<in> I\<^sub>C) minimalA minimalAC"
-unfolding minimalA_def minimal.minimal'_def
-apply (rule Corres_UL.corres_noop)
-apply wp
-apply (auto simp: no_fail_def R_def return_def)
-done
+definition
+  read_passphrase_rel :: "string TPM.STORED_DATA \<Rightarrow> tdTPM_STORED_DATA12_C \<times> lifted_globals \<Rightarrow> bool"
+where
+  "read_passphrase_rel d d' \<equiv> True"
 
-lemma refines: "AC_minimal \<sqsubseteq> A_minimal"
+lemma read_passphrase_corres: "corres read_passphrase_rel \<top> \<top> read_passphrase read_passphrase'"
+unfolding read_passphrase_def read_passphrase'_def
+proof -
+  have "corres read_passphrase_rel \<top> \<top> (do x \<leftarrow> TPM_NV_ReadValue 4 0 None;
+                                          case x of Inl e \<Rightarrow> exit_r | Inr b \<Rightarrow> return b
+                                         od)
+       (do ret' \<leftarrow> (unknown >>= (\<lambda>au. TPM_NV_ReadValue' 4 0 0x190 (hasValue_C_update (\<lambda>_. 0) au) NULL));
+           (when (TPM_NV_ReadValue_ret_C.returnCode_C ret' \<noteq> 0) (exit' (TPM_NV_ReadValue_ret_C.returnCode_C ret')) >>=
+           (\<lambda>_. unpack_TPM_STORED_DATA12' (TPM_NV_ReadValue_ret_C.data_C ret') (TPM_NV_ReadValue_ret_C.dataSize_C ret')))
+        od)" (is "corres _ _ _ (?a >>= ?b) (?c >>= ?d)")
+  proof -
+    let ?r' = "TPM_NV_ReadValue_rel StoredData_rel"
+    let ?R = "\<top>\<top>"
+    let ?R' = "\<top>\<top>"
+    have "corres ?r' \<top> \<top> ?a ?c"
+    apply (rule corres_symb_exec_r [where Q'="\<lambda>_. PO'"])
+      using TPM_NV_ReadValue_corres [where P=\<top> and P'=\<top> and idx=4 and idx'=4 and off=0 and off'=0
+        and size'="0x190" and s'=NULL and a=None] unfolding comp_def apply simp
+      unfolding unknown_def apply (wp select_wp, simp)
+      apply clarsimp
+      apply (rule_tac Q="\<lambda>s\<^sub>C. (s\<^sub>A, s\<^sub>C) \<in> R" in hoare_weaken_pre)
+      apply (wp select_wp, simp_all)
+      apply (rule non_fail_select')
+    done
+    moreover have "\<And>rv rv'. corres read_passphrase_rel (?R rv) (\<lambda>s'. ?r' rv (rv', s') \<and> ?R' rv' s') (?b rv) (?d rv')"
+    proof (rule corres_assume_pre)
+      fix rv rv' s s'
+      assume G: "PO s \<and> True"
+         and G': "PO' s' \<and> TPM_NV_ReadValue_rel StoredData_rel rv (rv', s') \<and> True"
+         and "(s, s') \<in> R"
+      let ?corres_b_d = "corres read_passphrase_rel (?R rv) (\<lambda>s'. ?r' rv (rv', s') \<and> ?R' rv' s')
+                    (?b rv) (?d rv')"
+      { fix error
+        assume rv: "rv = Inl error"
+        with G' have rv': "TPM_NV_ReadValue_ret_C.returnCode_C rv' \<noteq> 0"
+          unfolding TPM_NV_ReadValue_rel_def ERROR_rel_def TPM_BASE_def by auto
+        have "corres \<top>\<top> \<top> \<top> exit (exit' (TPM_NV_ReadValue_ret_C.returnCode_C rv'))"
+          using exit_corres [where P=PO and P'=PO'] by auto
+        moreover have "corres read_passphrase_rel (\<lambda>s. \<not>(PO s))
+          (\<lambda>s'. ?r' rv (rv', s') \<and> \<not>(PO' s')) unknown
+            (unpack_TPM_STORED_DATA12' (TPM_NV_ReadValue_ret_C.data_C rv')
+             (TPM_NV_ReadValue_ret_C.dataSize_C rv'))"
+          by (simp add: corres_underlying_def)
+        moreover have "\<lbrace>\<top>\<rbrace> exit \<lbrace>\<rbrace>"
+        have ?corres_b_d sorry}
+      moreover
+      { fix val
+        assume rv: "rv = Inr val"
+        with G' have rv': "TPM_NV_ReadValue_ret_C.returnCode_C rv' = 0"
+          unfolding TPM_NV_ReadValue_rel_def ERROR_rel_def TPM_SUCCESS_def TPM_BASE_def by auto
+        have ?corres_b_d sorry}
+      ultimately show ?corres_b_d by (meson sum_all_ex(2))
+    hence 
+ (*   hence 
+      { fix error
+        assume "rv = Inl error"
+        hence "corres read_passphrase_rel \<top> (\<lambda>s'. TPM_NV_ReadValue_rel StoredData_rel rv (rv', s')) exit (?d rv')"
+  
+  proof (rule corres_split [where r'="\<lambda>s'. TPM_NV_ReadValue_rel StoredData_rel rv (rv', s')" and R="\<top>\<top>" and R'="\<top>\<top>"])
+    fix val val'
+    let ?goal = "corres (\<lambda>_ _. True) (\<lambda>_. True) (\<lambda>s'. True \<and> True) (case val of Inl e \<Rightarrow> exit | Inr b \<Rightarrow> return b)
+               (do _ \<leftarrow> when (TPM_NV_ReadValue_ret_C.returnCode_C val' \<noteq> 0) (exit' (TPM_NV_ReadValue_ret_C.returnCode_C val'));
+                   unpack_TPM_STORED_DATA12' (TPM_NV_ReadValue_ret_C.data_C val') (TPM_NV_ReadValue_ret_C.dataSize_C val')
+                od)"
+    { fix error
+      assume "val = Inl error"
+      hence "corres (\<lambda>_ _. True) (\<lambda>_. True) (\<lambda>s'. True) exit
+               (do _ \<leftarrow> when (TPM_NV_ReadValue_ret_C.returnCode_C val' \<noteq> 0) (exit' (TPM_NV_ReadValue_ret_C.returnCode_C val'));
+                   unpack_TPM_STORED_DATA12' (TPM_NV_ReadValue_ret_C.data_C val') (TPM_NV_ReadValue_ret_C.dataSize_C val')
+                od)"
+      have "?goal" }
+  sorry
+  thus "corres (\<lambda>_ _. True) (\<lambda>_. True) (\<lambda>_. True) (TPM_NV_ReadValue 4 0 None <catch> (\<lambda>e. exit))
+       (do nv_auth___struct_TPM_AUTHDATA_option_C \<leftarrow> unknown;
+           ret' \<leftarrow> TPM_NV_ReadValue' 4 0 0x190 (hasValue_C_update (\<lambda>_. 0) nv_auth___struct_TPM_AUTHDATA_option_C) NULL;
+           when (TPM_NV_ReadValue_ret_C.returnCode_C ret' \<noteq> 0) (exit' (TPM_NV_ReadValue_ret_C.returnCode_C ret'));
+           unpack_TPM_STORED_DATA12' (TPM_NV_ReadValue_ret_C.data_C ret') (TPM_NV_ReadValue_ret_C.dataSize_C ret')
+        od)" unfolding catch_def by (simp add: bind_assoc)
+qed*)
+
+(*lemma refines: "AC_minimal \<sqsubseteq> A_minimal"
 proof (rule sim_imp_refines)
   have "A_minimal \<Turnstile> I\<^sub>A" unfolding I\<^sub>A_def by auto
   moreover have "AC_minimal \<Turnstile> I\<^sub>C" unfolding I\<^sub>C_def by auto
@@ -36,5 +110,7 @@ proof (rule sim_imp_refines)
   ultimately show "AC_minimal \<sqsubseteq>\<^sub>F A_minimal"
     using LI_fw_sim and L_invariantI by blas
 qed*)
+
+end
 
 end
