Proofs/StateRelation.thy
@@ -1,0 +1,35 @@
+theory StateRelation
+imports
+  TPM_Relation
+  "../Abstract/Abstract"
+begin
+
+context sable_verified
+begin
+
+definition
+  TPM_SESSION_rel :: "(TPM.AUTHHANDLE \<times> Session) \<Rightarrow> tdTPM_SESSION_C \<Rightarrow> bool"
+where
+  "TPM_SESSION_rel x s' \<equiv> case x of (h, s) \<Rightarrow>
+    of_nat h = tdTPM_SESSION_C.authHandle_C s' \<and>
+    NONCE_rel (Session.nonceEven s) (tdTPM_SESSION_C.nonceEven_C s') \<and>
+    NONCE_rel (Session.nonceOdd s) (tdTPM_SESSION_C.nonceOdd_C s') \<and>
+    BOOL_rel (Session.continue s) (tdTPM_SESSION_C.continueAuthSession_C s')"
+
+definition
+  R :: "(astate \<times> lifted_globals) set"
+where
+  "R \<equiv> {(s, s'). (powerOn \<circ> machine) s \<and> (powerOn \<circ> phantom_machine_state_'') s' \<longrightarrow>
+       (let sess_deref = \<lambda>p'. heap_tdTPM_SESSION_C s' (heap_tdTPM_SESSION_C'ptr s' p') in
+       let sess_valid = \<lambda>p'. is_valid_tdTPM_SESSION_C'ptr s' p' \<and> is_valid_tdTPM_SESSION_C s'
+              (heap_tdTPM_SESSION_C'ptr s' p') in
+         Ball (set (array_addrs (Ptr (symbol_table ''sessions'')) 2))
+             (\<lambda>p'. sess_valid p'
+             \<longrightarrow> (\<forall>sess. \<exists>h. sessions s h = Some sess \<and> TPM_SESSION_rel (h, sess) (sess_deref p')))
+         \<and> (\<forall>sess h. sessions s h = Some sess \<longrightarrow>
+              Bex (set (array_addrs (Ptr (symbol_table ''sessions'')) 2))
+             (\<lambda>p'. sess_valid p' \<and> TPM_SESSION_rel (h, sess) (sess_deref p'))))}"
+
+end
+
+end
