Proofs/TPM_Relation.thy
@@ -1,6 +1,6 @@
 theory TPM_Relation
 imports
-  "../Abstract/TPM"
+  "../Machine/TPM"
   "../AutoCorres/Impl"
 begin
 
@@ -65,8 +65,107 @@ value "RESULT_rel (Inr ()) 1" (* False *)
 value "RESULT_rel (Inl AUTHFAIL) 1" (* True *)
 
 definition
-  DIGEST_rel :: "TPM.DIGEST \<Rightarrow> tdTPM_DIGEST_C \<Rightarrow> bool"
+  BOOL_rel :: "bool \<Rightarrow> 8 word \<Rightarrow> bool"
 where
-  "DIGEST_rel d d' \<equiv> True"
+  "BOOL_rel b b' \<equiv> b \<longleftrightarrow> b' \<noteq> 0"
+
+value "BOOL_rel True 14" (* True *)
+value "BOOL_rel False 14" (* False *)
+value "BOOL_rel False 0" (* True *)
+
+(* This relation is axiomatized *)
+consts DIGEST_rel :: "TPM.DIGEST \<Rightarrow> tdTPM_DIGEST_C \<Rightarrow> bool"
+
+(* This relation is axiomatized *)
+consts NONCE_rel :: "TPM.NONCE \<Rightarrow> tdTPM_NONCE_C \<Rightarrow> bool"
+
+(* This relation is axiomatized *)
+consts AUTHDATA_rel :: "TPM.AUTHDATA \<Rightarrow> tdTPM_AUTHDATA_C \<Rightarrow> bool"
+
+(* FIXME *)
+definition
+  ENTITY_TYPE_rel :: "TPM.ENTITY_TYPE \<Rightarrow> 16 word \<Rightarrow> bool"
+where
+  "ENTITY_TYPE_rel t t' \<equiv> True"
+
+definition
+  LOCALITY_rel :: "TPM.LOCALITY \<Rightarrow> 8 word \<Rightarrow> bool"
+where
+  "LOCALITY_rel l l' \<equiv>
+    case l of
+      LOC_ZERO \<Rightarrow> l' = 1 << 0
+    | LOC_ONE \<Rightarrow> l' = 1 << 1
+    | LOC_TWO \<Rightarrow> l' = 1 << 2
+    | LOC_THREE \<Rightarrow> l' = 1 << 3
+    | LOC_FOUR \<Rightarrow> l' = 1 << 4"
+
+definition
+  LOCALITY_SELECTION_rel :: "TPM.LOCALITY_SELECTION \<Rightarrow> 8 word \<Rightarrow> bool"
+where
+  "LOCALITY_SELECTION_rel l l' \<equiv> \<forall>loc \<in> l. \<exists>mask. LOCALITY_rel loc (l' AND mask)"
+
+(* FIXME *)
+definition
+  PCR_SELECTION_rel :: "TPM.PCR_SELECTION \<Rightarrow> tdTPM_PCR_SELECTION_C \<times> lifted_globals \<Rightarrow> bool"
+where
+  "PCR_SELECTION_rel p p' \<equiv> True"
+
+definition
+  PCR_INFO_LONG_rel :: "TPM.PCR_INFO_LONG \<Rightarrow> tdTPM_PCR_INFO_LONG_C \<times> lifted_globals \<Rightarrow> bool"
+where
+  "PCR_INFO_LONG_rel i i' \<equiv>
+    tdTPM_PCR_INFO_LONG_C.tag_C (fst i') = 6 \<and>
+    LOCALITY_SELECTION_rel (TPM.PCR_INFO_LONG.localityAtCreation i)
+      (tdTPM_PCR_INFO_LONG_C.localityAtCreation_C (fst i')) \<and>
+    LOCALITY_SELECTION_rel (TPM.PCR_INFO_LONG.localityAtRelease i)
+      (tdTPM_PCR_INFO_LONG_C.localityAtRelease_C (fst i')) \<and>
+    PCR_SELECTION_rel (TPM.PCR_INFO_LONG.creationPCRSelection i)
+      (tdTPM_PCR_INFO_LONG_C.creationPCRSelection_C (fst i'), snd i') \<and>
+    PCR_SELECTION_rel (TPM.PCR_INFO_LONG.releasePCRSelection i)
+      (tdTPM_PCR_INFO_LONG_C.releasePCRSelection_C (fst i'), snd i') \<and>
+    DIGEST_rel (TPM.PCR_INFO_LONG.digestAtCreation i)
+      (tdTPM_PCR_INFO_LONG_C.digestAtCreation_C (fst i')) \<and>
+    DIGEST_rel (TPM.PCR_INFO_LONG.digestAtRelease i)
+      (tdTPM_PCR_INFO_LONG_C.digestAtRelease_C (fst i'))"
+
+definition
+  PAYLOAD_TYPE_rel :: "PAYLOAD_TYPE \<Rightarrow> 8 word \<Rightarrow> bool"
+where
+  "PAYLOAD_TYPE_rel p p' \<equiv> case p of PT_SEAL \<Rightarrow> p' = 5"
+
+(* We don't care about this yet
+definition
+  SEALED_DATA_rel :: "(('a :: Hashable) \<Rightarrow> (8 word ptr \<times> 32 word) \<times> lifted_globals \<Rightarrow> bool)
+    \<Rightarrow> 'a TPM.SEALED_DATA
+    \<Rightarrow> tdTPM_SEALED_DATA_C \<times> lifted_globals \<Rightarrow> bool"
+where
+  "SEALED_DATA_rel vrel d d' \<equiv>
+    PAYLOAD_TYPE_rel (TPM.SEALED_DATA.payload d) (tdTPM_SEALED_DATA_C.payload_C (fst d')) \<and>
+    AUTHDATA_rel (TPM.SEALED_DATA.authData d) (tdTPM_SEALED_DATA_C.authData_C (fst d')) \<and>
+    AUTHDATA_rel (TPM.SEALED_DATA.tpmProof d) (tdTPM_SEALED_DATA_C.tpmProof_C (fst d')) \<and>
+    DIGEST_rel (TPM.SEALED_DATA.storedDigest d) (tdTPM_SEALED_DATA_C.storedDigest_C (fst d')) \<and>
+    vrel (TPM.SEALED_DATA.data d) ((tdTPM_SEALED_DATA_C.data_C (fst d'),
+      tdTPM_SEALED_DATA_C.dataSize_C (fst d')), snd d')"
+*)
+
+(* Bogus for now *)
+definition
+  STORED_DATA_rel :: "(('a :: Hashable) \<Rightarrow> (8 word ptr \<times> 32 word) \<times> lifted_globals \<Rightarrow> bool)
+    \<Rightarrow> 'a TPM.STORED_DATA \<Rightarrow> tdTPM_STORED_DATA12_C \<times> lifted_globals \<Rightarrow> bool"
+where
+  "STORED_DATA_rel vrel d d' \<equiv> True"
+
+(* Function return relations *)
+
+(* FIXME
+definition
+  ReadValue_STORED_DATA_rel :: "('a :: Hashable) TPM.STORED_DATA
+    \<Rightarrow> (8 word ptr \<times> 32 word) \<times> lifted_globals \<Rightarrow> bool"
+where
+  "ReadValue_STORED_DATA_rel d d' \<equiv>
+    let s' = snd d' in
+    let ptr' = fst (fst d') in
+    let size' = snd (fst d') in
+    vrel d " *)
 
 end
